\subsection{Proof of Lemma \eqref{lbl_lemma_excited_states_ONB}}\label{proof_lbl_lemma_excited_states_ONB}

\begin{lemma}[{\cite[Lemma 11.5]{Hall2013}}]
  Let $\alpha \in \C$ be any scalar. Then, the partial sums of the series
  \begin{equation*}
    \sum_{n=0}^{\infty} \frac{\alpha^n \tilde{x}^n}{n!}\exp\left(-\frac{\tilde{x}^2}{2}\right)
  \end{equation*}
  converge in $L^2(\R)$ to $\exp\left(\alpha \tilde{x}\right)\exp\left(-\frac{\tilde{x}^2}{2}\right)$.
\end{lemma}
\begin{proof}
  We showcase this proof directly from the proof of {\cite[Lemma 11.5]{Hall2013}}. We start by noting that $\exp\left(\abs{\alpha} \tilde{x}\right) \exp\left( -\frac{\tilde{x}^2}{2} \right)$ is non-negative for all $\tilde{x} \in \R$. Now,
  \begin{align*}
    &\norm{
      \exp\left(\alpha \tilde{x}\right) \exp\left( -\frac{\tilde{x}^2}{2} \right)
      -
      \sum_{n=0}^{N} \frac{(\alpha \tilde{x})^n}{n!} \exp\left( -\frac{\tilde{x}^2}{2} \right)
    }^2 \\
    &=
    \norm{
      \sum_{n=0}^{\infty} \left(\frac{(\alpha \tilde{x})^n}{n!} \exp\left( -\frac{\tilde{x}^2}{2} \right)\right)
      -
      \sum_{n=0}^{N} \left(\frac{(\alpha \tilde{x})^n}{n!} \exp\left( -\frac{\tilde{x}^2}{2} \right)\right)
    }^2 \\
    &=
    \norm{
      \sum_{n=N+1}^{\infty} \left(\frac{(\alpha \tilde{x})^n}{n!} \exp\left( -\frac{\tilde{x}^2}{2} \right)\right)
    }^2 \\
    &=
    \int_{-\infty}^{\infty} \abs{\sum_{n=N+1}^{\infty} \left(\frac{(\alpha \tilde{x})^n}{n!} \exp\left( -\frac{\tilde{x}^2}{2} \right)\right)}^2 \,\mathrm{d}\tilde{x}.
  \end{align*}
  As we have the pointwise convergence
  \begin{equation*}
    \sum_{n=0}^{\infty} \left(\frac{(\alpha \tilde{x})^n}{n!} \exp\left( -\frac{\tilde{x}^2}{2} \right)\right)
    =
    \exp\left(\alpha \tilde{x}\right) \exp\left( -\frac{\tilde{x}^2}{2} \right),
  \end{equation*}
  we must have that the tail of the series, \[\sum_{n=N+1}^{\infty} \left(\frac{(\alpha \tilde{x})^n}{n!} \exp\left( -\frac{\tilde{x}^2}{2} \right)\right),\] pointwise converges to 0 as $N \to \infty$. Now, we see that
  \begin{align*}
    \abs{\sum_{n=N+1}^{\infty} \left(\frac{(\alpha \tilde{x})^n}{n!} \exp\left( -\frac{\tilde{x}^2}{2} \right)\right)}
    &\leq
    \sum_{n=N+1}^{\infty} \abs{\frac{(\alpha \tilde{x})^n}{n!} \exp\left( -\frac{\tilde{x}^2}{2} \right)} \\
    &=
    \sum_{n = N+1}^{\infty} \frac{\abs{\alpha\tilde{x}}^n}{n!} \exp\left( -\frac{\tilde{x}^2}{2} \right) \\
    &=
    \sum_{n = 0}^{\infty} \frac{\abs{\alpha\tilde{x}}^n}{n!} \exp\left( -\frac{\tilde{x}^2}{2} \right) \\
    &=
    \exp\left( \abs{a}\abs{\tilde{x}} \right)\exp\left( -\frac{\tilde{x}^2}{2} \right).
  \end{align*}
  After a bit of fiddling, we end up with
  \begin{equation*}
    \abs{\sum_{n= N+1}^{\infty} \frac{(\alpha\tilde{x})^n}{n!} \exp\left(-\frac{\tilde{x}^2}{2} \right)}^2
    \leq
    \exp\left( 2 \abs{\alpha}\abs{\tilde{x}}\right) \exp\left( -\tilde{x}^2 \right).
  \end{equation*}
  Now, it can be seen that $\exp\left( 2\abs{\alpha}\abs{\tilde{x}}\right)\exp\left( -\tilde{x}^2 \right)$ has a finite valued integral by making an appropriate substitution and using Lemma \eqref{lbl_oscillator_hard_integral}. This means that, by the dominated convergence theorem, Theorem \eqref{lbl_thrm_dominated_convergence}, we get that
  \begin{align*}
    \norm{
    \exp\left(\alpha \tilde{x}\right) \exp\left(-\frac{\tilde{x}}{2}\right)
    -
    \sum_{n=0}^{\infty} \frac{\alpha^n \tilde{x}^n}{n!} \exp\left(-\frac{\tilde{x}^2}{2}\right)
    }^2
    \to 0
  \end{align*}
  as $N \to \infty$, giving us our result.
\end{proof}
