\subsection{Proof of Proposition \eqref{lbl_prop_quantum_harmonic_oscillator_ito_ladders}}\label{proof_lbl_prop_quantum_harmonic_oscillator_ito_ladders}

\begin{proposition}[{\cite[p.229]{Hall2013}}]
  The Hamiltonian $H \colon \mathcal{S}(\R) \to L^2(\R)$ for the quantum harmonic oscillator is given by
  \begin{equation*}
    H = \hbar \omega \left(a^* a + \frac{1}{2}I \right),
  \end{equation*}
  where $a$ and $a^*$ are also defined on $\mathcal{S}(\R)$.
\end{proposition}
\begin{proof}
  This calculation is done in {\cite[p.229]{Hall2013}}, and we repeat it here. Recall that one of the cannonical commutation relationships, Proposition \eqref{lbl_cannonical_commutation_relations}), tells us that $[X, P] = i \hbar I$. Now,
  \begin{align*}
    a^* a
    &= \frac{1}{2\hbar m \omega } (m \omega X - i P) (m \omega X + i P) \\
    &= \frac{1}{2 \hbar m \omega}\left( (m\omega X^2) + P^2 + [m \omega X, i P] \right) \\
    &= \frac{1}{2\hbar m \omega } \big( (m \omega X)^2 + P^2 + i m \omega [X, P] \big) \\
    &= \frac{1}{2\hbar m \omega } \big( (m \omega X)^2 + P^2 + i^2 m \omega \hbar I \big) \\
    &=\frac{1}{2\hbar m \omega } \big( (m \omega X)^2 + P^2 \big) - \frac{1}{2}I \\
    &= \frac{1}{\hbar \omega} H - \frac{1}{2}I.
  \end{align*}
  Re-arranging shows us that
  \begin{equation*}
    H = \hbar \omega \left(a^* a + \frac{1}{2}I \right).
  \end{equation*}
\end{proof}
