\subsection{Proof of Proposition \eqref{lbl_aastar_lowers_raises}}\label{proof_lbl_aastar_lowers_raises}

\begin{proposition}[{\cite[Proposition 11.1]{Hall2013}}]
  Suppose that $a^*a$ is defined on $\mathcal{S}(\R)$ and has an eigenvector $\psi$, and let $\lambda$ be the corresponding eigenvalue to $\psi$. Then,
  \begin{enumerate}[label=(\alph*)]
    \item $a^*a (a\psi) = (\lambda - 1)a\psi$.
    \item $a^*a (a^* \psi) = (\lambda + 1)a^*\psi$.
  \end{enumerate}
\end{proposition}
\begin{proof}
  This proof comes from the proof of {\cite[Proposition 11.1]{Hall2013}}. Let $\psi$ be an eigenvector for $a^*a$ with the corresponding eigenvalue $\lambda$. By Proposition \eqref{lbl_raising_commutation_relationships} we have that
  \begin{equation*}
    [a, a^*a] = a.
  \end{equation*}
  By definition of the commutator operator and our assumption that $\psi$ is an eigenvector of $a^*a$ with corresponding eigenvalue $\lambda$, we see that
  \begin{align*}
    a^*a(a\psi)
    &= (a(a^* a) - a) \psi \\
    &= a\lambda\psi - a\psi \\
    &= (\lambda - 1)a\psi.
  \end{align*}
  Analogously, by Proposition \eqref{lbl_raising_commutation_relationships} we also have that
  \begin{equation*}
    [a^*, a^*a] = -a^*,
  \end{equation*}
  so we get that
  \begin{align*}
    a^*a (a\psi)
    &= (a^*(a^*a) + a^*)\psi \\
    &= a^*\lambda\psi + a^*\psi \\
    &= (\lambda + 1)a^*\psi.
  \end{align*}
\end{proof}
