\subsection{Proof of Proposition \eqref{lbl_prop_commutator_properties}}\label{proof_lbl_prop_commutator_properties}

\begin{proposition}[{\cite[Proposition 3.15]{Hall2013}}]
  Let $S$, $T$, and $R$ be operators in $\HS$ defined on a common domain such that the range of each operator is contained in this domain. Then,
  \begin{enumerate}[label = (\alph*)]
    \item For all $\alpha \in \C$, $[S, T + \alpha R] = [S, T] + \alpha [S, R]$.
    \item $[S, T] = - [T, S]$.
    \item $[S, TR] = [S, T]R + T[S, R]$.
    \item $\big[ S, [T, R] \big] = \big[ [S, T], R \big] + \big[T, [S, R] \big]$.
  \end{enumerate}
\end{proposition}
\begin{proof}
  As the proof of {\cite[Proposition 3.15]{Hall2013}} points out, these are simple calculations reliant on our associativity and distributivity properties of operator addition and composition. For part (a), we see that for any $\alpha \in \C$,
  \begin{align*}
    [S, T + \alpha R]
    &=
    S(T + \alpha R) - (T + \alpha R)S \\
    &=
    ST + \alpha SR - TS - \alpha RS \\
    &=
    ST - TS + \alpha  (SR - RS) \\
    &=
    [S, T] + \alpha [S, R].
  \end{align*}
  For part (b), we see that
  \begin{align*}
    [S, T]
    &=
    ST - TS \\
    &=
    - (TS - ST) \\
    &=
    - [S, T].
  \end{align*}
  For part (c), we have that
  \begin{align*}
    [S, T]R + T[S, R]
    &=
    (ST - TS)R + T[SR - RS] \\
    &=
    STR - TSR + TSR - TRS \\
    &=
    STR - TRS \\
    &=
    [S, TR].
  \end{align*}
  Finally, for part (d), we see that
  \begin{align*}
    \big[S, [T, R]\big]
    &=
    [S, TR - RT] \\
    &=
    [S, TR] - [S, RT] & \text{by part (a)} \\
    &=
    [S, T]R + T[S, R] - [S, R]T - R[S, T] &\text{by part (c)} \\
    &=
    [S, T]R - R[S,T] + T[S, R] - [S, R]T \\
    &=
    \big[ [S, T], R \big] + \big[ T, [S, R]  \big].
  \end{align*}
\end{proof}
