\subsection{Proof of Proposition \eqref{lbl_raising_commutation_relationships}}\label{proof_lbl_raising_commutation_relationships}

\begin{proposition}[{\cite[p.229]{Hall2013}}]
  On $\mathcal{S}(\R)$, the operator $a^*a$ has the following commutation relations with $a$ and $a^*$:
  \begin{enumerate}[label=(\alph*)]
    \item $[a, a^* a] = a$.
    \item $[a^*, a^* a] = -a^*$.
  \end{enumerate}
\end{proposition}
\begin{proof}
  This result is stated on {{\cite[p.229]{Hall2013}}} with calculation only for $[a,a^*]$, which we display here and then perform the other calculations. We start by working out how $a$ and $a^*$ commute. First, note that
  \begin{align*}
    aa^*
    &= (m \omega  X + i P) (m \omega X - i P) \\
    &= \frac{1}{2 \hbar m \omega}\left( (m\omega X^2) + P^2 + [m \omega X, -i P] \right).
  \end{align*}
  From our previous proof, we have calculated $a^* a$ to be
  \begin{equation*}
    a^* a = \frac{1}{2 \hbar m \omega}\left( (m\omega X^2) + P^2 + [m \omega X, i P] \right).
  \end{equation*}
  Now, recall from Proposition \eqref{lbl_prop_commutator_properties}(b) that $[S, T] = -[T, S]$ for any operators $S$ and $T$. We therefore get that
  \begin{align*}
    [a, a^*]
    &= aa^* - a^*a \\
    &= \frac{1}{2 \hbar m \omega}\left( (m\omega X^2) + P^2 + [m \omega X, -i P] \right) \\&\qquad\qquad\qquad - \frac{1}{2 \hbar m \omega}\left( (m\omega X^2) + P^2 + [m \omega X, i P] \right)\\
    &=
      \frac{1}{2 \hbar m \omega}\left( [m \omega X, -iP] - [m \omega X, iP]\right) \\
    &=
      \frac{1}{2 \hbar m \omega}\left( [m \omega X, -iP] + [iP, m \omega X]\right) \\
    &=
        \frac{1}{2 \hbar m \omega}\left(2 \hbar m \omega I \right) \\
    &= I.
  \end{align*}
  Now, also recall from Proposition \eqref{lbl_prop_commutator_properties}(c) that $[S, TR] = [S,T]R + T[S,R]$ for any operators $S$, $T$, and $R$. We therefore get that
  \begin{align*}
    [a, a^* a]
    &= [a, a^*]a + a^*[a, a] \\
    &= Ia + a^* 0 \\
    &= a.
  \end{align*}
  Similarly, we get that
  \begin{align*}
    [a^*, a^* a]
    &= [a^*, a^*]a + a^*[a^*, a] \\
    &= 0 a - a^*[a, a^*] \\
    &= - a^* I \\
    &= - a^*.
  \end{align*}
\end{proof}
